simulations/simglobal/SimGlobalFacts.v
@@ -65,12 +65,12 @@ Section ADEQUACY.
 
   Section MAIN.
     Variable md_src md_tgt: Mod.t.
-    Let ms_src: ModSem.t := md_src.(Mod.enclose).
-    Let ms_tgt: ModSem.t := md_tgt.(Mod.enclose).
+    Let ms_src: ModSem.t := Mod.enclose md_src.
+    Let ms_tgt: ModSem.t := Mod.enclose md_tgt.
     Hypothesis (SIM: simg eq false false (@ModSem.initial_itr ms_src (Mod.wf md_src)) (@ModSem.initial_itr ms_tgt (Mod.wf md_tgt))).
 
     Theorem adequacy_global:
-      Beh.of_program (@Mod.compile _ md_tgt) <1= Beh.of_program (@Mod.compile _ md_src).
+      Beh.of_program (@Mod.compile md_tgt) <1= Beh.of_program (@Mod.compile md_src).
     Proof.
       eapply adequacy_global_itree. eapply SIM.
     Qed.
